Cleaner proofs through refactoring

Valaig/FinMC/Basic.lean
@@ -50,45 +50,60 @@ an array) such that each pair are related by the transition relation.
 -/
 structure FinPath {α : Type} (ts : TransSys α) where
   states : Array α
-  sized : states.size ≠ 0
+  sized : states.size > 0
 
   trans :
     ∀ {i : Nat} (_ : i < states.size - 1),
       ts.trans states[i] states[i + 1]
 
-attribute [grind .] FinPath.sized
+attribute [local grind! .] FinPath.sized
+attribute [local grind .] FinPath.trans
 
 namespace FinPath
+variable {path : FinPath ts}
 
-abbrev size (path : FinPath ts) : Nat :=
+def size (path : FinPath ts) : Nat :=
   path.states.size
 
-instance {path : FinPath ts} : NeZero (path.size) := by
-  rw [neZero_iff]
-  exact path.sized
+@[simp, grind! .]
+theorem zero_lt_size :
+    0 < path.size := by
+  grind [size]
 
-abbrev state (path : FinPath ts) (idx : Nat) (bound : idx < path.size := by get_elem_tactic) : α :=
+instance : NeZero (path.size) := by
+  grind [neZero_iff, size]
+
+def state (path : FinPath ts) (idx : Nat) (lt_size : idx < path.size := by grind) : α :=
   path.states[idx]
+
+/--
+The index of `final`.
+-/
+@[simp]
+abbrev lastIdx (path : FinPath ts) : Nat :=
+  path.size - 1
 
 /--
 The initial state of a path is the state with the lowest index.
 -/
 def initial (path : FinPath ts) : α :=
-  have := path.sized
-  path.states[0]
+  path.states[0]'path.sized
+
+@[simp, grind =]
+theorem initial_def :
+    path.initial = path.state 0 := by
+  simp [initial, state]
 
 /--
 The final state of a path is the state with the greatest index.
 -/
 def final (path : FinPath ts) : α :=
-  have := path.sized
-  path.states.back
+  path.states.back (by grind only [path.sized])
 
-/--
-The index of `final`.
--/
-abbrev lastIdx (path : FinPath ts) : Nat :=
-  path.size - 1
+@[simp, grind =]
+theorem final_def :
+    path.final = path.state path.lastIdx := by
+  simp [final, Array.back_eq_getElem, state, size]
 
 /--
 A path between two states is a path such that the initial and final states
@@ -96,18 +111,6 @@ are these states.
 -/
 def Between (path : FinPath ts) (initial final : α) : Prop :=
   path.initial = initial ∧ path.final = final
-
-/--
-A path is simple if it does not visit the same state twice.
--/
-@[expose, reducible, simp]
-def Simple (path : FinPath ts) : Prop :=
-  ∀ {i j : Nat} (_ : i < path.size) (_ : j < path.size),
-    i ≠ j →
-      path.state i ≠ path.state j
-
-abbrev SimplePath {α : Type} (ts : TransSys α) :=
-  { path : FinPath ts // path.Simple }
 
 /--
 Construct a trivial path from a single state.
@@ -119,19 +122,205 @@ def trivial (state : α) : FinPath ts :=
     trans := by simp
   }
 
+section trivial
+variable {state : α}
+
+@[simp, grind =]
+theorem size_trivial :
+    (trivial state : FinPath ts).size = 1 := by
+  simp [trivial, size]
+
+@[simp, grind =]
+theorem state_zero_trivial :
+    (trivial state : FinPath ts).state 0 = state := by
+  simp [trivial, FinPath.state]
+
+@[simp, grind =]
+theorem state_trivial {idx : Nat} (eq_zero : idx = 0) :
+    (trivial state : FinPath ts).state idx = state := by
+  simp [eq_zero]
+
+@[simp]
+theorem initial_trivial :
+    (trivial state : FinPath ts).initial = state := by
+  simp
+
+@[simp]
+theorem final_trivial :
+    (trivial state : FinPath ts).final = state := by
+  grind
+
+end trivial
+
 /--
 Add a new state to the end of the path that obeys the transition relation.
 -/
-def push (path : FinPath ts) (state : α) (trans : ts.trans path.final state := by grind) :
-    FinPath ts :=
+def push (path : FinPath ts) (state : α) (trans : ts.trans path.final state := by grind) : FinPath ts :=
   {
     states := path.states.push state,
     sized := by simp,
-    trans := by grind [FinPath.trans, final]
+    trans := by grind [FinPath.trans, size, state]
   }
 
+section push
+variable {state : α} {trans : ts.trans path.final state}
+
+@[simp, grind =]
+theorem size_push :
+    (path.push state trans).size = path.size + 1 := by
+  simp [push, size]
+
+@[simp]
+theorem state_push_lt {idx : Nat} (h : idx < path.size) :
+    (path.push state trans).state idx = path.state idx := by
+  grind [push, size, state]
+
+@[simp]
+theorem state_push_eq :
+    (path.push state trans).state path.size = state:= by
+  simp [push, size, FinPath.state]
+
+@[grind =]
+theorem state_push {idx : Nat} (h : idx < (path.push state trans).size) :
+    (path.push state trans).state idx =
+    if h : idx < path.size then
+      path.state idx
+    else
+      state := by
+  simp [push, size, FinPath.state, Array.getElem_push]
+
+@[simp]
+theorem initial_push :
+    (path.push state trans).initial = path.initial := by
+  grind
+
+@[simp]
+theorem final_push :
+    (path.push state trans).final = state := by
+  grind
+
+end push
+
+/--
+Extract the subsequence of the path from `start` to `stop` exclusive.
+-/
+def extract (path : FinPath ts) (start stop : Nat)
+    (le_stop : start < stop := by grind)
+    (le_size : stop ≤ path.size := by grind) : FinPath ts :=
+  {
+    states := path.states.extract start stop,
+    sized := by simp_all [size],
+    trans := by grind
+  }
+
+section extract
+variable {start stop : Nat} (le_stop : start < stop) (le_size: stop ≤ path.size)
+
+@[simp, grind =]
+theorem size_extract :
+    (path.extract start stop le_stop le_size).size = stop - start := by
+  grind [extract, size]
+
+@[simp, grind =]
+theorem state_extract {i : Nat} (h : i < (path.extract start stop le_stop le_size).size) :
+    (path.extract start stop le_stop le_size).state i = path.state (start + i) := by
+  simp [extract, state]
+
+@[simp]
+theorem initial_extract :
+    (path.extract start stop le_stop le_size).initial = path.state start := by
+  simp_all
+
+@[simp]
+theorem final_extract :
+    (path.extract start stop le_stop le_size).final = path.state (stop - 1) := by
+  grind
+
+end extract
+
+/--
+Truncate the path to size `size`.
+-/
+def truncate (path : FinPath ts) (size : Nat)
+    (zero_lt : 0 < size := by grind)
+    (le_size : size ≤ path.size := by grind) : FinPath ts :=
+  path.extract 0 size
+
+section truncate
+variable {size : Nat} (zero_lt : 0 < size) (le_size : size ≤ path.size)
+
+@[local grind =]
+theorem truncate_eq_extract :
+    path.truncate size zero_lt le_size = path.extract 0 size := by
+  simp [truncate]
+
+@[simp, grind =]
+theorem size_truncate :
+    (path.truncate size zero_lt le_size).size = size := by
+  grind
+
+@[simp, grind =]
+theorem state_truncate {i : Nat} (h : i < size) :
+    (path.truncate size zero_lt le_size).state i = path.state i := by
+  grind
+
+@[simp]
+theorem initial_truncate :
+    (path.truncate size zero_lt le_size).initial = path.initial := by
+  simp_all
+
+@[simp]
+theorem final_truncate :
+    (path.truncate size zero_lt le_size).final = path.state (size - 1) := by
+  simp_all
+
+end truncate
+
+/--
+For every path there is a shorter path with the same initial state.
+-/
+theorem exists_shorter_path_initial_eq {size : Nat} (leSize : size ≤ path.size) (gtZero : size > 0) :
+    ∃ (path' : FinPath ts) (_ : path'.size = size),
+      path'.initial = path.initial := by
+  exists path.truncate size
+  grind 
+
+/--
+For every path there is a shorter path with the same final state.
+-/
+theorem exists_shorter_path_final_eq {size : Nat} (leSize : size ≤ path.size) (gtZero : size > 0) :
+    ∃ (path' : FinPath ts) (_ : path'.size = size),
+      path'.final = path.final := by
+    exists path.extract (path.size - size) path.size
+    grind
+
+/--
+A path is simple if it does not visit the same state twice.
+-/
+@[grind]
+def Simple (path : FinPath ts) : Prop :=
+  ∀ {i j : Nat} (_ : i < path.size) (_ : j < path.size),
+    i ≠ j →
+      path.state i ≠ path.state j
+
+section simple
+variable {state : α} {trans : ts.trans path.final state}
+
+@[simp, grind .]
+theorem Simple_trivial :
+    (trivial state : FinPath ts).Simple := by
+  grind
+
+@[simp, grind .]
+theorem Simple_push_of_Simple (simple : path.Simple)
+    (new : ∀ {idx} (_ : idx < path.size), path.state idx ≠ state) :
+    (path.push state trans).Simple := by
+  grind
+
+end simple
+
 namespace removeLoops
-variable [DecidableEq α] {path : FinPath ts} {idx : Nat} {bound : idx < path.size}
+variable [DecidableEq α] {idx : Nat} {lt_size : idx < path.size}
 variable {state : α}
 
 /--
@@ -139,7 +328,7 @@ Returns the greatest index in `path` that is equal to `state` and at most `idx`,
 if one exists.
 -/
 private def findIdx [DecidableEq α] (path : FinPath ts)
-    (state : α) (idx : Nat) (bound : idx < path.size := by lia) : Option Nat :=
+    (state : α) (idx : Nat) (lt_size : idx < path.size := by lia) : Option Nat :=
   if path.state idx = state then
     some idx
   else if h : idx = 0 then
@@ -148,7 +337,7 @@ private def findIdx [DecidableEq α] (path : FinPath ts)
     findIdx path state (idx - 1)
 
 private theorem findIdx_lt :
-    match findIdx path state idx bound with
+    match findIdx path state idx lt_size with
     | some n => n ≤ idx
     | _ => True := by
   fun_induction findIdx
@@ -157,7 +346,7 @@ private theorem findIdx_lt :
   · grind only [Option.all_eq_true]
 
 private theorem findIdx_eq :
-    match _ : findIdx path state idx bound with
+    match _ : findIdx path state idx lt_size with
     | some n =>
       path.state n (by grind only [findIdx_lt]) = state
     | _ => True := by
@@ -165,10 +354,8 @@ private theorem findIdx_eq :
   <;> grind only [findIdx]
 
 private theorem findIdx_eq_none_implies_forall_ne :
-    match _ : findIdx path state idx bound with
-    | none =>
-      ∀ {idx' : Nat} (_ : idx' ≤ idx), path.state idx' ≠ state
-    | _ => True := by
+    (h : findIdx path state idx lt_size = none) →
+      ∀ {idx' : Nat} (_ : idx' ≤ idx), path.state idx' ≠ state := by
   fun_induction findIdx
   · simp
   · grind only
@@ -176,10 +363,10 @@ private theorem findIdx_eq_none_implies_forall_ne :
 
 private def removeUpTo
     [DecidableEq α] (path : FinPath ts) (idx : Nat)
-    (bound : idx < path.size := by grind) :
+    (lt_size : idx < path.size := by grind) :
     { path' : FinPath ts // path'.final = path.state idx } :=
   if hidx : idx = 0 then
-    ⟨.trivial path.initial, by simp_all [final, FinPath.state, initial, trivial]⟩
+    ⟨.trivial path.initial, by simp_all⟩
   else
     let state := path.state idx
     match h : removeLoops.findIdx path state (idx - 1) with
@@ -188,42 +375,54 @@ private def removeUpTo
       ⟨removeUpTo path j, by grind only [findIdx_eq]⟩
     | none =>
       let pre := removeUpTo path (idx - 1)
-      have trans := by grind only [trans]
+      have trans := by grind [trans, size, state]
       let path' := pre.val.push state trans
-      have h := by simp [path', push, final, state, Array.back_eq_getElem]
+      have h := by simp [path', state]
       ⟨path', h⟩
 termination_by idx
 
 private theorem removeUpTo_initial_eq_initial :
-    (removeUpTo path idx bound).val.initial = path.initial := by
+    (removeUpTo path idx lt_size).val.initial = path.initial := by
   fun_induction removeUpTo
-  · simp [initial, trivial]
+  · simp
   · simpa
-  · grind [push, initial]
+  · grind
 
 private theorem removeUpTo_size_le :
-    (removeUpTo path idx bound).val.size ≤ idx + 1 := by
+    (removeUpTo path idx lt_size).val.size ≤ idx + 1 := by
   fun_induction removeUpTo
-  · simp [initial, trivial, size]
+  · simp
   · lia
-  · grind [push]
+  · grind
 
 private theorem removeUpTo_subset_states :
-    let path' := removeUpTo path idx bound
+    let path' := removeUpTo path idx lt_size
     ∀ {newIdx : Nat} (_ : newIdx < path'.val.size),
       ∃ (oldIdx : Nat) (_ : oldIdx ≤ idx),
         path'.val.state newIdx = path.state oldIdx := by
   fun_induction removeUpTo
-  · simp [trivial, size, initial]; grind
-  · grind only
-  · grind [push, removeUpTo_size_le]
+  <;> grind [removeUpTo]
+
+private theorem findIdx_eq_none_implies_removeUpTo_ne_state :
+    findIdx path state idx lt_size = none →
+    let path' := removeUpTo path idx lt_size
+    ∀ {newIdx : Nat} (_ : newIdx < path'.val.size),
+      path'.val.state newIdx ≠ state := by
+  intro h _ _ size
+  rcases removeUpTo_subset_states size with ⟨_, ⟨newSize, _⟩⟩
+  have := findIdx_eq_none_implies_forall_ne h newSize
+  grind only
 
 private theorem removeUpTo_Simple :
-    (removeUpTo path idx bound).val.Simple := by
+    (removeUpTo path idx lt_size).val.Simple := by
   fun_induction removeUpTo
-  · grind [trivial, initial]
+  · grind
   · simpa
-  · grind [removeUpTo_subset_states, push, findIdx_eq_none_implies_forall_ne, final]
+  next ih1 ih2 =>
+    apply Simple_push_of_Simple
+    · assumption
+    · assumption
+    · grind only [findIdx_eq_none_implies_removeUpTo_ne_state]
 
 end removeLoops
 
@@ -248,7 +447,7 @@ theorem removeLoops_initial_eq :
 
 theorem removeLoops_final_eq :
     path.removeLoops.final = path.final := by
-  grind only [removeLoops, final, Array.back_eq_getElem]
+  grind only [removeLoops, final_def]
 
 theorem removeLoops_Simple :
     path.removeLoops.Simple := by
@@ -262,13 +461,11 @@ set_option linter.unusedVariables false in
 For all finite paths, there exists a simple path between the same states
 that is at most as long (by removing the loops).
 -/
-theorem exists_simple_path [DecidableEq α] :
-    ∀ (path : FinPath ts),
+theorem exists_simple_path [DecidableEq α] (path : FinPath ts) :
     ∃ (path' : FinPath ts)
       (ends : path'.Between path.initial path.final)
       (simple : path'.Simple),
       path'.size ≤ path.size := by
-  intro path
   exists path.removeLoops
   apply Exists.intro ?_
   apply Exists.intro ?_
@@ -287,14 +484,12 @@ cardinality of the domain (as any longer path must revisit states).
 We show this by creating an injective mapping from path indices to states, where
 the path indices have a cardinality of `path.size`.
 -/
-theorem size_le_card_of_finite_simple [Finite α] :
-  ∀ (path : FinPath ts) (simple : path.Simple),
+theorem size_le_card_of_finite_simple [Finite α] (simple : path.Simple) :
     path.size ≤ Nat.card α := by
-  intro path simple
   rw [←Nat.card_fin path.size]
   let map : Fin path.size -> α := (path.state ·)
   apply Nat.card_le_card_of_injective map
-  grind only [Function.Injective]
+  grind [Function.Injective]
 
 end FinPath
 
@@ -321,7 +516,7 @@ theorem Safe_iff_not_reachable_not :
 
 set_option linter.unusedVariables false in
 def SafeUpTo (ts : TransSys α) (pred : α -> Prop) (bound : Nat) :=
-  ∀ (trace : FinTrace ts) (upto : trace.size ≤ bound),
+  ∀ (trace : FinTrace ts) (lt_bound : trace.size ≤ bound),
     pred trace.final
 
 variable {pred : α -> Prop}
@@ -344,7 +539,7 @@ theorem Safe_iff_SafeUpTo_card_of_finite [Finite α] [DecidableEq α] :
         toFinPath := simplePath,
         init := by grind [FinTrace.init]
       }
-    have := FinPath.size_le_card_of_finite_simple simplePath simple
+    have := FinPath.size_le_card_of_finite_simple simple
     have : trace.final = trace'.final := by grind
     rw [this]
     apply h
